fv/lean/Ragu/Circuits/Element/Mul.lean
@@ -20,35 +20,35 @@ def main (input : Var Input (F p)) : Circuit (F p) (Var field (F p)) := do
   assertZero (y - input.y)
   return z
 
-def Assumptions (_input : Input (F p)) (_data : ProverData (F p)) :=
+def Assumptions (_input : Input (F p)) :=
   True
 
-def Spec (input : Input (F p)) (out : field (F p)) (_data : ProverData (F p)) :=
+def Spec (input : Input (F p)) (out : field (F p)) :=
   out = input.x * input.y
 
 instance elaborated : ElaboratedCircuit (F p) Input field where
   main := main
   localLength _ := 3
 
-theorem soundness : GeneralFormalCircuit.Soundness (F p) elaborated Spec := by
+theorem soundness : Soundness (F p) elaborated Assumptions Spec := by
   circuit_proof_start
   obtain ⟨c1, c2, c3⟩ := h_holds
   rw [add_neg_eq_zero] at c1 c2 c3
   rw [←c2, ←c3, c1]
 
-theorem completeness : GeneralFormalCircuit.Completeness (F p) elaborated Assumptions := by
+theorem completeness : Completeness (F p) elaborated Assumptions := by
   circuit_proof_start
   have h0 := h_env (0 : Fin 3)
   have h1 := h_env (1 : Fin 3)
   have h2 := h_env (2 : Fin 3)
-  simp only [toElements, circuit_norm, explicit_provable_type, Core.AllocMul.Row, List.sum] at h0 h1 h2
+  simp only [toElements, circuit_norm, explicit_provable_type, List.sum] at h0 h1 h2
   norm_num at h0 h1 h2
   simp at h0 h1 h2
   rw [show i₀ + 1 + 1 = i₀ + 2 from by omega]
   rw [h0, h1, h2]
   refine ⟨?_, ?_, ?_⟩ <;> ring
 
-def circuit : GeneralFormalCircuit (F p) Input field :=
+def circuit : FormalCircuit (F p) Input field :=
   {
     elaborated with
     Assumptions,
