fv/lean/Ragu/Instances/Point/AddIncomplete.lean
@@ -100,7 +100,7 @@ def formal_instance : Core.Statements.FormalInstance where
   same_constraints := by
     intro input
     simp [Core.Statements.FlatOperation.eraseCompute, List.map,
-      Operations.toFlat, circuit_norm, GeneralFormalCircuit.toSubcircuit,
+      Operations.toFlat, circuit_norm, GeneralFormalCircuit.toSubcircuit, FormalCircuit.toSubcircuit,
       deserializeInput, exportedOperations,
       Circuits.Point.AddIncomplete.circuit, Circuits.Point.AddIncomplete.elaborated, Circuits.Point.AddIncomplete.main,
       Circuits.Element.Square.circuit, Circuits.Element.Square.elaborated, Circuits.Element.Square.main,
@@ -110,7 +110,7 @@ def formal_instance : Core.Statements.FormalInstance where
     constructor
   same_output := by
     intro input;
-    simp [circuit_norm, GeneralFormalCircuit.toSubcircuit,
+    simp [circuit_norm, GeneralFormalCircuit.toSubcircuit, FormalCircuit.toSubcircuit,
       deserializeInput, serializeOutput,
       Circuits.Point.AddIncomplete.circuit, Circuits.Point.AddIncomplete.elaborated, Circuits.Point.AddIncomplete.main,
       Circuits.Element.Square.circuit, Circuits.Element.Square.elaborated, Circuits.Element.Square.main,
