fv/lean/Ragu/Instances/Point/AllocFq.lean
@@ -65,10 +65,7 @@ def formal_instance : Core.Statements.FormalInstance where
     intro input
     simp [Core.Statements.FlatOperation.eraseCompute, List.map,
       Operations.toFlat, circuit_norm, GeneralFormalCircuit.toSubcircuit,
-      Circuits.Point.Alloc.circuit, Circuits.Point.Alloc.elaborated, Circuits.Point.Alloc.main,
-      Circuits.Core.AllocMul.circuit, Circuits.Core.AllocMul.elaborated, Circuits.Core.AllocMul.main,
-      Circuits.Element.AllocSquare.circuit, Circuits.Element.AllocSquare.elaborated, Circuits.Element.AllocSquare.main,
-      Circuits.Element.Mul.circuit, Circuits.Element.Mul.elaborated, Circuits.Element.Mul.main]
+      Circuits.Point.Alloc.circuit, Circuits.Point.Alloc.elaborated, Circuits.Point.Alloc.main]
     rfl
   same_output := by intro input; rfl
   same_spec := by intro input output; rfl
