fv/lean/Ragu/Instances/Point/Double.lean
@@ -79,7 +79,7 @@ def formal_instance : Core.Statements.FormalInstance where
   same_constraints := by
     intro input
     simp [Core.Statements.FlatOperation.eraseCompute, List.map,
-      Operations.toFlat, circuit_norm, GeneralFormalCircuit.toSubcircuit,
+      Operations.toFlat, circuit_norm, GeneralFormalCircuit.toSubcircuit, FormalCircuit.toSubcircuit,
       deserializeInput, exportedOperations,
       Circuits.Point.Double.circuit, Circuits.Point.Double.elaborated, Circuits.Point.Double.main,
       Circuits.Element.Square.circuit, Circuits.Element.Square.elaborated, Circuits.Element.Square.main,
@@ -89,7 +89,7 @@ def formal_instance : Core.Statements.FormalInstance where
     constructor
   same_output := by
     intro input;
-    simp [circuit_norm, GeneralFormalCircuit.toSubcircuit,
+    simp [circuit_norm, GeneralFormalCircuit.toSubcircuit, FormalCircuit.toSubcircuit,
       deserializeInput, serializeOutput,
       Circuits.Point.Double.circuit, Circuits.Point.Double.elaborated, Circuits.Point.Double.main,
       Circuits.Element.Square.circuit, Circuits.Element.Square.elaborated, Circuits.Element.Square.main,
